update

Test/civl/regression-tests/funky.bpl
@@ -1,122 +1,122 @@
 // RUN: %parallel-boogie "%s" > "%t"
 // RUN: %diff "%s.expect" "%t"
-type {:linear "tid"} X;
+type {:linear} X;
 const nil: X;
 
 var {:layer 0,3} A: X;
 var {:layer 0,3} B: X;
 var {:layer 0,3} counter: int;
-var {:layer 0,3}{:linear "tid"} unallocated:[X]bool;
+var {:layer 0,3}{:linear} unallocated: Set X;
 
-right action {:layer 1,3} AtomicLockA({:linear "tid"} tid: X)
+right action {:layer 1,3} AtomicLockA({:linear} tid: One X)
 modifies A;
-{ assert tid != nil; assume A == nil; A := tid; }
+{ assert tid->val != nil; assume A == nil; A := tid->val; }
 
-yield procedure {:layer 0} LockA({:linear "tid"} tid: X);
+yield procedure {:layer 0} LockA({:linear} tid: One X);
 refines AtomicLockA;
 
-right action {:layer 1} AtomicIncrA({:linear "tid"} tid: X)
+right action {:layer 1} AtomicIncrA({:linear} tid: One X)
 modifies counter;
-{ assert tid != nil && A == tid; counter := counter + 1; }
+{ assert tid->val != nil && A == tid->val; counter := counter + 1; }
 
-yield procedure {:layer 0} IncrA({:linear "tid"} tid: X);
+yield procedure {:layer 0} IncrA({:linear} tid: One X);
 refines AtomicIncrA;
 
-right action {:layer 1} AtomicDecrA({:linear "tid"} tid: X)
+right action {:layer 1} AtomicDecrA({:linear} tid: One X)
 modifies counter;
-{ assert tid != nil && A == tid; counter := counter - 1; }
+{ assert tid->val != nil && A == tid->val; counter := counter - 1; }
 
-yield procedure {:layer 0} DecrA({:linear "tid"} tid: X);
+yield procedure {:layer 0} DecrA({:linear} tid: One X);
 refines AtomicDecrA;
 
-left action {:layer 1,3} AtomicUnlockA({:linear "tid"} tid: X)
+left action {:layer 1,3} AtomicUnlockA({:linear} tid: One X)
 modifies A;
-{ assert tid != nil && A == tid; A := nil; }
+{ assert tid->val != nil && A == tid->val; A := nil; }
 
-yield procedure {:layer 0} UnlockA({:linear "tid"} tid: X);
+yield procedure {:layer 0} UnlockA({:linear} tid: One X);
 refines AtomicUnlockA;
 
-right action {:layer 1,3} AtomicLockB({:linear "tid"} tid: X)
+right action {:layer 1,3} AtomicLockB({:linear} tid: One X)
 modifies B;
-{ assert tid != nil; assume B == nil; B := tid; }
+{ assert tid->val != nil; assume B == nil; B := tid->val; }
 
-yield procedure {:layer 0} LockB({:linear "tid"} tid: X);
+yield procedure {:layer 0} LockB({:linear} tid: One X);
 refines AtomicLockB;
 
-atomic action {:layer 1,2} AtomicIncrB({:linear "tid"} tid: X)
+atomic action {:layer 1,2} AtomicIncrB({:linear} tid: One X)
 modifies counter;
-{ assert tid != nil && B == tid; counter := counter + 1; }
+{ assert tid->val != nil && B == tid->val; counter := counter + 1; }
 
-yield procedure {:layer 0} IncrB({:linear "tid"} tid: X);
+yield procedure {:layer 0} IncrB({:linear} tid: One X);
 refines AtomicIncrB;
 
-atomic action {:layer 1} AtomicDecrB({:linear "tid"} tid: X)
+atomic action {:layer 1} AtomicDecrB({:linear} tid: One X)
 modifies counter;
-{ assert tid != nil && B == tid; counter := counter - 1; }
+{ assert tid->val != nil && B == tid->val; counter := counter - 1; }
 
-yield procedure {:layer 0} DecrB({:linear "tid"} tid: X);
+yield procedure {:layer 0} DecrB({:linear} tid: One X);
 refines AtomicDecrB;
 
-left action {:layer 1,3} AtomicUnlockB({:linear "tid"} tid: X)
+left action {:layer 1,3} AtomicUnlockB({:linear} tid: One X)
 modifies B;
-{ assert tid != nil && B == tid; B := nil; }
+{ assert tid->val != nil && B == tid->val; B := nil; }
 
-yield procedure {:layer 0} UnlockB({:linear "tid"} tid: X);
+yield procedure {:layer 0} UnlockB({:linear} tid: One X);
 refines AtomicUnlockB;
 
-atomic action {:layer 1,3} AtomicAssertA({:linear "tid"} tid: X)
-{ assert tid != nil && A == tid; assert counter >= -1; }
+atomic action {:layer 1,3} AtomicAssertA({:linear} tid: One X)
+{ assert tid->val != nil && A == tid->val; assert counter >= -1; }
 
-yield procedure {:layer 0} AssertA({:linear "tid"} tid: X);
+yield procedure {:layer 0} AssertA({:linear} tid: One X);
 refines AtomicAssertA;
 
-atomic action {:layer 1,3} AtomicAssertB({:linear "tid"} tid: X)
-{ assert tid != nil && A == tid && B == tid; assert counter == 0; }
+atomic action {:layer 1,3} AtomicAssertB({:linear} tid: One X)
+{ assert tid->val != nil && A == tid->val && B == tid->val; assert counter == 0; }
 
-yield procedure {:layer 0} AssertB({:linear "tid"} tid: X);
+yield procedure {:layer 0} AssertB({:linear} tid: One X);
 refines AtomicAssertB;
 
-right action {:layer 1,3} AtomicAllocTid() returns ({:linear "tid"} tid: X)
+right action {:layer 1,3} AtomicAllocTid() returns ({:linear} tid: One X)
 modifies unallocated;
 {
-  assume tid != nil;
-  assume unallocated[tid];
-  unallocated[tid] := false;
+  var x: X;
+  assume x != nil && Set_Contains(unallocated, x);
+  call tid := One_Get(unallocated, x);
 }
 
-yield procedure {:layer 0} AllocTid() returns ({:linear "tid"} tid: X);
+yield procedure {:layer 0} AllocTid() returns ({:linear} tid: One X);
 refines AtomicAllocTid;
 
-right action {:layer 2} AtomicAbsDecrB({:linear "tid"} tid: X)
+right action {:layer 2} AtomicAbsDecrB({:linear} tid: One X)
 modifies counter;
-{ assert tid != nil && B == tid && counter == 0; counter := counter - 1; }
+{ assert tid->val != nil && B == tid->val && counter == 0; counter := counter - 1; }
 
-yield procedure {:layer 1} AbsDecrB({:linear "tid"} tid: X)
+yield procedure {:layer 1} AbsDecrB({:linear} tid: One X)
 refines AtomicAbsDecrB;
 {
     call DecrB(tid);
 }
 
-both action {:layer 3} AtomicAbsAssertA({:linear "tid"} tid: X)
-{ assert tid != nil && A == tid; assert counter >= -1; }
+both action {:layer 3} AtomicAbsAssertA({:linear} tid: One X)
+{ assert tid->val != nil && A == tid->val; assert counter >= -1; }
 
-yield procedure {:layer 2} AbsAssertA({:linear "tid"} tid: X)
+yield procedure {:layer 2} AbsAssertA({:linear} tid: One X)
 refines AtomicAbsAssertA;
 {
     call AssertA(tid);
 }
 
-both action {:layer 3} AtomicAbsAssertB({:linear "tid"} tid: X)
-{ assert tid != nil && A == tid && B == tid; assert counter == 0; }
+both action {:layer 3} AtomicAbsAssertB({:linear} tid: One X)
+{ assert tid->val != nil && A == tid->val && B == tid->val; assert counter == 0; }
 
-yield procedure {:layer 2} AbsAssertB({:linear "tid"} tid: X)
+yield procedure {:layer 2} AbsAssertB({:linear} tid: One X)
 refines AtomicAbsAssertB;
 {
     call AssertB(tid);
 }
 
-yield procedure {:layer 1} TA({:linear "tid"} tid: X)
-requires {:layer 1} tid != nil;
+yield procedure {:layer 1} TA({:linear} tid: One X)
+requires {:layer 1} tid->val != nil;
 {
     call LockA(tid);
     call IncrA(tid);
@@ -124,10 +124,10 @@ requires {:layer 1} tid != nil;
     call UnlockA(tid);
 }
 
-both action {:layer 3} AtomicTB({:linear "tid"} tid: X)
-{ assert tid != nil && counter == 0; }
+both action {:layer 3} AtomicTB({:linear} tid: One X)
+{ assert tid->val != nil && counter == 0; }
 
-yield procedure {:layer 2} TB({:linear "tid"} tid: X)
+yield procedure {:layer 2} TB({:linear} tid: One X)
 refines AtomicTB;
 {
     call LockB(tid);
@@ -136,18 +136,18 @@ refines AtomicTB;
     call UnlockB(tid);
 }
 
-yield procedure {:layer 3} AbsTB({:linear "tid"} tid: X)
-requires {:layer 3} tid != nil;
+yield procedure {:layer 3} AbsTB({:linear} tid: One X)
+requires {:layer 3} tid->val != nil;
 requires call YieldCounter();
 {
     call TB(tid);
 }
 
-yield procedure {:layer 3} main({:linear "tid"} tid: X)
-requires {:layer 3} tid != nil;
+yield procedure {:layer 3} main({:linear} tid: One X)
+requires {:layer 3} tid->val != nil;
 requires call YieldCounter();
 {
-    var {:linear "tid"} cid: X;
+    var {:linear} cid: One X;
 
     while (*)
     invariant {:yields} true;
