Test/civl/regression-tests/bernhard1.bpl
@@ -1,13 +1,12 @@
 // RUN: %parallel-boogie "%s" > "%t"
 // RUN: %diff "%s.expect" "%t"
 
-type {:linear "x"} X = int;
-var {:linear "x"} {:layer 0,1} A : [int]bool;
+var {:linear} {:layer 0,1} A : Set int;
 
-yield procedure {:layer 1} Proc ({:linear "x"} i: int)
+yield procedure {:layer 1} Proc ({:linear} i: One int)
 {
   call {:layer 1} Lemma(A, i);
 }
 
-pure procedure Lemma (set: [int]bool, i: int);
-requires !set[i];
+pure procedure Lemma (set: Set int, i: One int);
+requires !Set_Contains(set, i->val);
